CBOR.Pulse.Raw.Format.Serialize.cbor_size

src/cbor/pulse/raw/CBOR.Pulse.Raw.Format.Serialize.fsti
@@ -21,3 +21,25 @@ val cbor_serialize
       SZ.v res == Seq.length s /\
       (exists v' . v `Seq.equal` (s `Seq.append` v'))
     ))
+
+noextract [@@noextract_to "krml"]
+let cbor_size_post
+  (bound: SZ.t)
+  (y: raw_data_item)
+  (res: SZ.t)
+: Tot prop
+=
+      let s = Seq.length (serialize_cbor y) in
+      (SZ.v res == 0 <==> s > SZ.v bound) /\
+      (SZ.v res > 0 ==> SZ.v res == s)
+
+val cbor_size
+  (x: cbor_raw)
+  (bound: SZ.t)
+  (#y: Ghost.erased raw_data_item)
+  (#pm: perm)
+: stt SZ.t
+    (cbor_match pm x y)
+    (fun res -> cbor_match pm x y ** pure (
+      cbor_size_post bound y res
+    ))
